replace the old reduction module with partial reduction module
We now have a completeness result for partial reduction, which subsumes
the result on total reduction.

Coq/Reduction.v
@@ -1,158 +1,649 @@
-Require Export Denotational.
+Require Export Specialise.
+Require Import Denotational.
 Require Import TranslateExp.
 Require Import Tactics.
 Require Import FunctionalExtensionality.
+Require Export FinMap.
+Require Import TimedTyping.
 
-(********** Reduction semantics **********)
+
+(********** reduction semantics **********)
+
+(* This is the reduction relation *)
 
 
-
-Inductive Red : Contr -> Env -> ExtEnv -> Contr -> Trans -> Prop :=
-| red_zero env ext : Red Zero env ext Zero empty_trans
-| red_let e env ext c c' t v :  E[| e |] env ext = Some v -> Red c (v::env) ext c' t ->
-               Red (Let e c) env ext (Let (translateExp (-1) e) c') t
-| red_transf c p1 p2 env ext : Red (Transfer c p1 p2) env ext Zero (singleton_trans c p1 p2 1)
-| red_scale e env ext c c' t v :  E[| e |] env ext = Some (RVal v) -> Red c env ext c' t ->
-               Red (Scale e c) env ext (Scale (translateExp (-1) e) c') (scale_trans v t)
-| red_trans0 c env ext c' t : Red c env ext c' t -> Red (Translate 0 c) env ext c' t
-| red_transS c env ext n : Red (Translate (S n) c) env ext (Translate n c) empty_trans
-| red_both c1 c1' c2 c2' env ext t1 t2 : Red c1 env ext c1' t1 -> Red c2 env ext c2' t2 -> 
-                         Red (Both c1 c2) env ext (Both c1' c2') (add_trans t1 t2)
-| red_if0_false env ext c1 c2 c' b t : E[|b|] env ext = Some (BVal false) -> 
-                                        Red c2 env ext c' t -> Red (If b 0 c1 c2) env ext c' t
-| red_ifS_false env ext c1 c2 n b : E[|b|] env ext = Some (BVal false) -> Red (If b (S n) c1 c2) env ext (If b n c1 c2) empty_trans
-| red_if_true env ext c1 c2 c' n b t : E[|b|] env ext = Some (BVal true) -> Red c1 env ext c' t -> Red (If b n c1 c2) env ext c' t
+Inductive ScaleTrans : option R -> Trans -> Trans -> Prop :=
+| scaleTrans_empty e : ScaleTrans e empty_trans empty_trans
+| scaleTrans_scale v t : ScaleTrans (Some v) t (scale_trans v t)
 .
+
+Inductive Red : Contr -> EnvP -> ExtEnvP -> Contr -> Trans -> Prop :=
+| red_zero env ext t c :t = empty_trans -> c = Zero -> Red Zero env ext c t
+| red_let e e' env ext c c' c'' t : e' = specialiseExp e env ext ->
+                                     Red c (fromLit e'::env) ext c' t ->
+                                     c'' = (smartLet (translateExp (-1) e') c') ->
+                                    Red (Let e c) env ext c'' t
+| red_transf c c' t' p1 p2 env ext : c' = Zero -> t' = (singleton_trans c p1 p2 1) -> Red (Transfer c p1 p2) env ext c' t'
+| red_scale e e' env ext c c' c'' t t' : e' = specialiseExp e env ext -> 
+                                   ScaleTrans (fromRLit e') t t' -> Red c env ext c' t ->
+                                   c'' = (smartScale (translateExp (-1) e') c') ->
+                                   Red (Scale e c) env ext c'' t'
+| red_trans0 c env ext c' t : Red c env ext c' t -> Red (Translate 0 c) env ext c' t
+| red_transS c env ext n c' t' : t' = empty_trans -> c' = Translate n c -> Red (Translate (S n) c) env ext c' t'
+| red_both c1 c1' c2 c2' env ext t1 t2 c t : Red c1 env ext c1' t1 -> Red c2 env ext c2' t2 -> 
+                                             c = smartBoth c1' c2' -> t = add_trans t1 t2 ->
+                                             Red (Both c1 c2) env ext c t
+| red_if0_false env ext c1 c2 c' b t : fromBLit (specialiseExp b env ext) = Some false -> 
+                                         Red c2 env ext c' t -> Red (If b 0 c1 c2) env ext c' t
+| red_ifS_false env ext c1 c2 n b c t : fromBLit (specialiseExp b env ext) = Some false -> 
+                                    c = If b n c1 c2 -> t = empty_trans -> 
+                                       Red (If b (S n) c1 c2) env ext c t
+| red_if_true env ext c1 c2 c' n b t : fromBLit (specialiseExp b env ext) = Some true -> 
+                                         Red c1 env ext c' t -> Red (If b n c1 c2) env ext c' t
+.
+
+(* N.B. If rule red_ifS_false used (specialiseExp b env ext) for the
+result contract, the rule would be unsound. *)
 
 Hint Constructors Red.
 
-Open Scope nat.
-
-Theorem red_sound1 c c' env ext tr t  : Red c env ext c' t ->  C[|c|] env ext = Some tr -> tr 0 = t.
+Theorem red_sound1 c c' env ext envp extp tr t g: 
+  g |-C c ->
+      TypeEnv g env -> TypeExt ext -> 
+  Red c envp extp c' t ->  
+  ext_inst extp ext ->
+  env_inst envp env ->
+  C[|c|] env ext = Some tr -> tr O = t.
 Proof.
-  intro R. generalize dependent tr. induction R; simpl; intros tr T. 
-  - inversion T. reflexivity.
-  - rewrite H in T. simpl in T. apply IHR. apply T.
-  - inversion T. reflexivity.
-  - rewrite H in T. option_inv' T. unfold scale_trace,compose.
-    simpl in H1. inversion H1. apply IHR in H2. subst. reflexivity.
-  - unfold delay_trace in T. simpl in T. rewrite adv_ext_0 in T.
-    option_inv' T. apply IHR. assumption.
-  - simpl in T. option_inv' T. reflexivity.
-  - option_inv' T. unfold add_trace. rewrite IHR1 by assumption. rewrite IHR2 by assumption. reflexivity.
-  - rewrite H in T. auto.
-  - rewrite H in T. option_inv' T. reflexivity.
-  - destruct n; simpl in *; rewrite H in T; auto.
+
+  Ltac spec := repeat match goal with 
+                  | [T: fromRLit _ = Some _ |- _ ] => apply fromRLit_fromLit in T
+                  | [T: fromBLit _ = Some _ |- _ ] => apply fromBLit_fromLit in T
+                  | [T: fromLit _ = Some _ |- _ ] => eapply specialise_fromLit in T;eauto; try rewrite T in *
+               end.
+  intros T E X R I J S. 
+  generalize dependent env. generalize dependent ext. generalize dependent g. generalize dependent tr.
+  induction R;intros; simpl in S; try option_inv' S; try solve [inversion S;auto|auto];inversion T;clear T;subst.
+  - eapply IHR;eauto. eauto using Esem_typed  . constructor. intros.
+    spec. inversion H3. reflexivity. assumption.
+  - unfold scale_trace,compose. option_inv_auto. erewrite IHR;eauto. inversion H0. 
+    * apply scale_empty_trans.
+    * symmetry in H3. spec. inversion H1. subst. simpl in H2. inversion H2. reflexivity.
+  - erewrite <- IHR;eauto. rewrite adv_ext_0 in H1. rewrite delay_trace_0. assumption.
+  - unfold add_trace. erewrite <- IHR1;eauto. erewrite <- IHR2;eauto.
+  - spec. eapply IHR;eauto. 
+  - spec. option_inv_auto. reflexivity.
+  - spec. eapply IHR;eauto. destruct n; simpl in S; rewrite H in S;assumption.
 Qed.
 
-Theorem red_sound2 c c' i env ext t t1 t2 : 
-  Red c env ext c' t -> C[|c|]env ext = Some t1 -> C[|c'|] env (adv_ext 1 ext) = Some t2
+
+Theorem red_typed c c' envp extp t g:
+  TypeEnvP g envp -> TypeExtP extp -> 
+  g |-C c -> Red c envp extp c' t ->  g |-C c'.
+Proof.
+  intros T1 T2 T R. generalize dependent g.
+  induction R;intros;inversion T;subst;
+  eauto 10 using smartLet_typed, smartBoth_typed, smartScale_typed, translateExp_type,specialiseExp_typed, fromLit_typed.
+Qed.
+
+Theorem red_sound2 c c' env ext envp extp t t1 t2 i g: 
+  g |-C c ->
+      TypeEnv g env -> TypeExt ext -> 
+  Red c envp extp c' t ->  
+  ext_inst extp ext ->
+  env_inst envp env ->
+  C[|c|]env ext = Some t1 -> C[|c'|] env (adv_ext 1 ext) = Some t2
   -> t1 (S i) = t2 i.
 Proof.
-  intros R T1 T2. generalize dependent t1. generalize dependent t2. induction R; simpl;intros.
-  - inversion T1. inversion T2. reflexivity.
-  - rewrite translateExp_ext in T2. rewrite adv_ext_iter in T2. simpl in T2. rewrite adv_ext_0 in T2.
-    rewrite H in *. simpl in *. apply IHR; auto.
-  - inversion T1. inversion T2. subst. reflexivity.
-  - rewrite translateExp_ext in T2. rewrite adv_ext_iter in T2. simpl in T2. rewrite adv_ext_0 in T2.
-    rewrite H in *. simpl in *. option_inv' T1. option_inv' T2. unfold pure,compose in *.
-    eapply IHR in H4;eauto. inversion H3. inversion H5. unfold scale_trace, compose in *. rewrite H4. 
-    reflexivity.
-  - unfold delay_trace in *. rewrite adv_ext_0 in T1. 
-    option_inv' T1. simpl. apply IHR; auto. 
-  - option_inv' T1. option_inv' T2.
-    unfold delay_trace in *. simpl in *. rewrite adv_ext_iter in H2. 
-    assert (Z.pos (Pos.of_succ_nat n) = (1 + Z.of_nat n)%Z).
-    assert (1%Z = Z.of_nat 1) by reflexivity. rewrite H in *.
-    rewrite <- Nat2Z.inj_add in *. reflexivity.
-    rewrite H in *.  rewrite H1 in H2. inversion H2. reflexivity.
-  - option_inv' T1. option_inv' T2. unfold add_trace. erewrite IHR1;eauto. erewrite IHR2;eauto.
-  - rewrite H in *. auto.
-  - unfold delay_trace in *. rewrite H in *. option_inv' T1. simpl in *. 
-    rewrite T2 in H2. inversion H2. f_equal. omega.
-  - destruct n; simpl in T1; rewrite H in T1; auto.
-Qed.
+  intros T E X R I J S1 S2. generalize dependent t1. generalize dependent t2. generalize dependent env. 
+  generalize dependent ext. generalize dependent g.
+  induction R; simpl in *;intros;inversion T;clear T;subst;try solve [inversion S1;inversion S2;eauto].
+  - option_inv_auto. eapply IHR;eauto. 
+    eauto using Esem_typed.  
+    constructor. intros. spec. inversion H0. reflexivity. auto. 
+    erewrite smartLet_sound in S2;eauto. simpl in S2. option_inv_auto.
+    rewrite translateExp_ext_opp in H2 by reflexivity.
+    erewrite specialiseExp_sound in H2;eauto. rewrite H2 in H0. inversion H0. subst. auto.
+  - option_inv_auto. spec. erewrite smartScale_sound in S2 by eauto 10 using red_typed.
+    simpl in S2. option_inv_auto. rewrite translateExp_ext_opp in H8 by reflexivity.
+    erewrite specialiseExp_sound in H8;eauto. 
+    unfold scale_trace, compose. erewrite IHR by eauto. f_equal. 
+    rewrite H8 in H3. inversion H3. subst. rewrite H9 in H4. inversion H4. reflexivity.
+  - option_inv_auto. rewrite delay_trace_0. eapply IHR;eauto.
+  - option_inv_auto. simpl in S2. option_inv_auto. rewrite delay_trace_S. f_equal.  rewrite adv_ext_iter in H1.
+    rewrite Zpos_P_of_succ_nat in H0. rewrite Z.add_1_l in H1. rewrite H0 in H1. inversion H1. reflexivity.
+  - option_inv_auto. erewrite smartBoth_sound in S2;eauto.
+    * simpl in S2. option_inv_auto. unfold add_trace,compose. f_equal;eauto.
+    * eauto 10 using red_typed.
+  - spec. eapply IHR;eauto.
+  - spec. option_inv_auto. rewrite delay_trace_S. rewrite delay_trace_0. simpl in S2.
+    rewrite H1 in S2. inversion S2. reflexivity.
+  - spec. eapply IHR;eauto. destruct n; simpl in S1; rewrite H in S1; assumption.
+    Qed.
 
-Ltac eauto_destruct := repeat(match goal with [ H : exists _, _ |- _] => destruct H end); eauto.
+Open Scope time.
 
-Theorem red_complete c env ext t : C[|c|] env ext = Some t -> exists c', Red c env ext c' (t 0).
+Definition ext_def_until (ext : ExtEnvP) t := 
+  forall l i, Time i <= t -> exists v, ext l i = Some v.
+
+Definition env_def_until (env : EnvP) ts t := 
+  all2 (fun v t' => time t' <= t -> exists v', v = Some v' /\ TypeVal v' (type t')) env ts.
+
+
+Lemma fromLit_toLit v : fromLit (toLit v) = Some v.
 Proof.
-  generalize dependent t. generalize dependent env. induction c; simpl; intros.
-  - inversion H. eauto.
-  - option_inv' H. apply IHc in H3. eauto_destruct.
-  - inversion H. simpl. eauto.
-  - option_inv' H. apply IHc in H2. destruct H2. 
-    unfold scale_trace, compose in *. option_inv' H1. destruct x2; tryfalse. 
-    simpl in *. inversion H4. subst. eauto.
-  - unfold delay_trace in *. option_inv' H. destruct n; simpl in *.
-    + rewrite adv_ext_0 in H2. apply IHc in H2. eauto_destruct.
-    + eauto.
-  -  unfold add_trace in *. option_inv' H. apply IHc1 in H1. apply IHc2 in H2.
-     eauto_destruct.
-  - remember (E[|e|]env ext) as B. destruct B as [b'| ]. 
-    + destruct b'. destruct b.
-      * destruct n; simpl in *; rewrite <- HeqB in *; apply IHc1 in H;
-        eauto_destruct. 
-      * destruct n; simpl in *;rewrite <- HeqB in *.
-        apply IHc2 in H. eauto_destruct.
-        unfold delay_trace in H. simpl in *. option_inv' H. eauto_destruct.
-      * destruct n; simpl in H; rewrite <- HeqB in *; tryfalse.
-    + destruct n; simpl in *; rewrite <- HeqB in *; inversion H.
+  destruct v;reflexivity.
+Qed.
+
+Lemma lookupEnvP_complete env tis ti v t:  
+  time ti <= t -> env_def_until env tis t -> TiTyV tis ti v
+  -> exists v', lookupEnvP v env = Some v' /\ TypeVal v' (type ti).
+Proof.
+  intros M E T. generalize dependent env. 
+  induction T;intros;
+  inversion E; subst; simpl; try rewr_assumption; eauto.
 Qed.
 
 
-Fixpoint RedFun (c : Contr) (env : Env) (ext : ExtEnv) : option (Contr * Trans) :=
-  match c with
-    | Zero => Some (Zero, empty_trans)
-    | Let e c => E[|e|]env ext >>= fun val => liftM (fun res : (Contr * Trans) => 
-                                                        let (c', t) := res in (Let (translateExp (-1) e) c', t)) 
-                                                     (RedFun c (val::env) ext)
-    | Transfer c p1 p2 => Some (Zero, singleton_trans c p1 p2 1)
-    | Scale e c => match RedFun c env ext, E[|e|]env ext with
-                       | Some (c', t), Some (RVal v) => Some (Scale (translateExp (-1) e) c', scale_trans v t)
-                       | _, _ => None
-                   end
-    | Translate l c => match l with
-                      | O => RedFun c env ext
-                      | S l' => Some (Translate l' c, empty_trans)
-                    end
-    | Both c1 c2 => match RedFun c1 env ext, RedFun c2 env ext with
-                      | Some (c1', t1), Some (c2', t2) => Some (Both c1' c2', add_trans t1 t2)
-                      | _, _ => None
-                    end
-    | If b l c1 c2 => match E[|b|] env ext with
-                              | Some (BVal false) => match l with
-                                                | O => RedFun c2 env ext
-                                                | S l' => Some (If b l' c1 c2, empty_trans)
-                                              end
-                              | Some (BVal true) => RedFun c1 env ext
-                              | _ => None
+Lemma add_time_0 t : add_time 0 t = t.
+Proof.
+  destruct t. destruct ti; simpl; try rewrite Z.add_0_r; reflexivity. 
+Qed.
+
+Lemma map_add_time_0 ts : map (add_time 0) ts = ts.
+Proof.
+  erewrite map_ext. apply map_id. intros. auto using add_time_0.
+Qed.
+
+
+Lemma adv_ext_def_until ext t d : 
+  ext_def_until ext t ->
+  ext_def_until (adv_ext (- Z.of_nat d) ext) (tadd' d t).
+Proof.
+  unfold ext_def_until. intros E. intros l i L. unfold adv_ext.
+  assert (Time (- Z.of_nat d + i) <= t) as L'
+  by (destruct t; simpl in *;inversion L; subst; constructor; omega).
+  eapply E in L'. decompose [ex] L'. rewr_assumption. eauto.
+Qed.
+
+Lemma add_time_tle s t d : tadd' d s <= tadd' d t -> s <= t.
+Proof.
+  intro T. destruct s, t; simpl in *;inversion T;subst;constructor;omega.
+Qed.
+
+Lemma env_def_until_add_time d env ti tis :  
+  env_def_until env tis ti
+  -> env_def_until env (map (add_time d) tis) (tadd' d ti).
+Proof.
+  unfold env_def_until. intros.
+  rewrite <- map_id with (l:=env). apply all2_map'. eapply all2_impl in H. 
+  apply H. simpl. intros. rewrite type_add_time. rewrite time_add_time in *.
+  eauto using add_time_tle.
+Qed.
+
+
+Lemma ext_def_until_adv d ext ti : 
+  (d <= 0)%Z -> ext_def_until ext ti -> ext_def_until (adv_ext d ext) ti.
+Proof.
+  unfold ext_def_until. intros L E l i Tl. 
+  assert (Time (d+i) <= ti) as Tl' by (inversion Tl; subst; constructor; omega).
+  eauto.
+Qed.
+
+Lemma ext_def_until_step ext ti : ext_def_until ext ti -> ext_def_until (adv_ext (-1) ext) ti.
+Proof.
+  intros. apply ext_def_until_adv. omega. assumption.
+Qed.
+
+
+
+(* Lemma all2_all : all2 P l1 l2 -> all (fun x => P) l2 *)
+
+(*  H5 : all2 (TiTyE tis) ts' args *)
+(*   H : all *)
+(*         (fun x : Exp => *)
+(*          TiTyE tis ti x -> *)
+(*          exists v : Val, *)
+(*            fromLit (specialiseExp x env ext) = Some v /\ |-V v ∶ type ti) *)
+(*         args *)
+
+Lemma ext_def_until_tle t t' ext : t' <= t -> ext_def_until ext t -> ext_def_until ext t'.
+Proof.
+  unfold ext_def_until. eauto. 
+Qed.
+
+Lemma env_def_until_tle ts t t' env : t' <= t -> env_def_until env ts t -> env_def_until env ts t'.
+Proof.
+  unfold env_def_until. intros l T. induction T;eauto.
+Qed.
+
+Lemma fromLit_real x : (exists v, fromLit x = Some v /\ TypeVal v REAL) -> exists v, x = OpE (RLit v) nil.
+Proof.
+  intro E. destruct E as [v E]. destruct E as [E1 E2]. inversion E2. subst.
+  apply toLit_fromLit in E1. subst. simpl. eauto.
+Qed.
+
+Lemma fromLit_bool x : (exists v, fromLit x = Some v /\ TypeVal v BOOL) -> exists v, x = OpE (BLit v) nil.
+Proof.
+  intro E. destruct E as [v E]. destruct E as [E1 E2]. inversion E2. subst.
+  apply toLit_fromLit in E1. subst. simpl. eauto.
+Qed.
+
+
+Ltac inv := match goal with
+              | [T : all2 _  _ _ |- _] => inversion T; clear T;subst
+              | [T : _ |- _] => first [apply fromLit_bool in T|apply fromLit_real in T];
+                               let x := fresh in destruct T as [x T];rewrite T;clear T
+              | [t : Ty |- _] => destruct t
+              | [ |- context[match ?x with _ => _ end]] => destruct x
+end.
+Lemma specialiseOp_complete ts ti args op env ext : 
+  |-Op op ∶ ts => ti
+  -> all2 (fun (e' : Exp) t' =>
+             exists v : Val,
+               fromLit (specialiseExp e' env ext) = Some v /\ |-V v ∶ t')  args ts
+  -> exists v,  (specialiseOp op (map (fun e' : Exp => specialiseExp e' env ext) args)) >>= fromLit = Some v
+               /\ TypeVal v ti.
+Proof.
+  intros TO As. destruct TO;repeat (inv;subst; simpl;eauto).
+Qed.
+
+Lemma specialiseExp_complete t tis ti e ext env : 
+  time ti <= t -> TiTyE tis ti e -> ext_def_until ext t -> env_def_until env tis t -> TypeExtP ext
+  -> exists v, fromLit (specialiseExp e env ext) = Some v /\ TypeVal v (type ti).
+Proof.
+  intros M T Ti E TE. 
+  generalize dependent env.   generalize dependent ext. 
+  generalize dependent ti. generalize dependent tis. generalize t.
+  induction e using Exp_ind';intros.
+  - inversion T. subst. clear T. simpl.
+    assert (all2 (fun e' t' => exists v, fromLit (specialiseExp e' env ext) = Some v
+                                               /\ TypeVal v t') args (map type ts')) as G.
+    inversion H4. subst. clear H4 H1.
+    induction H5;constructor.
+    + inversion H. inversion H0. subst. eapply H4;eauto; rewr_assumption;
+      eauto using ext_def_until_tle, env_def_until_tle.
+    + inversion H0. inversion H. subst. apply IHall2;  eauto. 
+    + clear H. inversion H4. eapply specialiseOp_complete in G;eauto.
+      destruct G as [v G]. destruct G as [G1 G2]. option_inv G1. rewr_assumption.
+      simpl. eauto.
+  - inversion T. subst. assert (exists v, ext l i = Some v) as D by eauto.
+    decompose [ex] D. simpl. rewr_assumption. simpl. 
+    assert (TypeVal' (ext l i) (type ti)) as T' by eauto.
+    rewr_assumption in T'. inversion T'. eauto using fromLit_toLit. 
+  - assert (exists v', lookupEnvP v env = Some v' /\ TypeVal v' (type ti)) as Hv
+      by (inversion T; subst; eauto using lookupEnvP_complete).
+    decompose [ex and] Hv. simpl. rewr_assumption. simpl. eauto using fromLit_toLit.
+  - simpl. inversion T. subst. clear T. pose Ti as Ti'.
+    apply adv_ext_def_until with (d:=d) in Ti'. 
+    eapply IHe2 in Ti';try rewrite time_add_time; eauto using env_def_until_add_time.
+    decompose [ex and] Ti'. clear Ti'. rewrite type_add_time in *. rewr_assumption. 
+    assert (exists v : Val,
+             Acc_sem
+                (specialiseFun (specialiseExp e1) env
+                   (adv_ext (- Z.of_nat d) ext)) d 
+                (Some x) = Some v /\ |-V v ∶ type ti) as G.
+    clear H0 H3.
+    generalize dependent env. generalize dependent ext. induction d;intros. 
+    + simpl in *. eauto.
+    + simpl. pose E as E'. eapply IHd with (ext:=adv_ext (-1) ext) in E';eauto using ext_def_until_step.
+      decompose [ex and] E'. repeat rewrite adv_ext_step'.
+      rewr_assumption. unfold specialiseFun.
+      eapply all2_cons with (y:=type ti @ TimeBot) in E;eauto. 
+      eapply IHe1 in E;eauto.
+      rewrite H0 in *. auto. rewrite <- adv_ext_step. rewrite adv_ext_opp by omega. assumption. 
+    + decompose [ex and] G. rewr_assumption. simpl. eauto using fromLit_toLit. 
+Qed.
+  
+Lemma tsub'_0 t: tsub' 0 t = t.
+Proof.
+  destruct t;simpl;f_equal. omega. reflexivity.
+Qed.
+
+Lemma map_sub_time_0 ts : map (sub_time 0) ts = ts.
+Proof.
+  erewrite map_ext. apply map_id. intros. destruct a. destruct ti; simpl; repeat f_equal. omega.
+Qed.
+
+Lemma fromLit_fromRLit e : 
+  (exists v, fromLit e = Some v /\ TypeVal v REAL)
+  -> exists r, fromRLit e = Some r.
+Proof.
+  intro E. decompose [ex and] E. destruct e;tryfalse. destruct op, args;tryfalse;simpl in *;eauto.
+  inversion H0. subst. inversion H1. 
+Qed.
+
+
+Lemma fromLit_fromBLit e : 
+  (exists v, fromLit e = Some v /\ TypeVal v BOOL)
+  -> exists b, fromBLit e = Some b.
+Proof.
+  intro E. decompose [ex and] E. destruct e;tryfalse. destruct op, args;tryfalse;simpl in *;eauto.
+  inversion H0. subst. inversion H1. 
+Qed.
+
+
+Definition mk_env_inst : TyEnv -> EnvP -> Env := 
+  zipWith (fun t v => match v with
+                  | Some v' => v'
+                  | None => match t with
+                              | BOOL => BVal false
+                              | REAL => RVal 0
                             end
+                      end).
+
+Lemma mk_env_inst_env_inst env tys : TypeEnvP tys env -> env_inst env (mk_env_inst tys env).
+Proof.
+  intros T. induction T;constructor;eauto. intros. destruct x; congruence.
+Qed.
+
+
+Lemma mk_env_inst_typed env tys : TypeEnvP tys env -> TypeEnv tys (mk_env_inst tys env).
+Proof.
+  intros T. induction T;constructor;eauto. intros. destruct x. inversion H. auto.
+  destruct y;eauto.
+Qed.  
+
+Definition mk_ext_inst (ext : ExtEnvP) : ExtEnv
+  := fun l i => match ext l i with
+                  | Some v => v
+                  | None => match l with
+                              | LabB _ => BVal false
+                              | LabR _ => RVal 0
+                            end
+                end.
+
+
+Lemma mk_ext_inst_ext_inst ext : ext_inst ext (mk_ext_inst ext).
+Proof.
+  unfold ext_inst, mk_ext_inst. intros. rewr_assumption. reflexivity.
+Qed.
+
+
+Lemma mk_ext_inst_typed ext: TypeExtP ext -> TypeExt (mk_ext_inst ext).
+Proof.
+  unfold TypeExt, TypeExtP, mk_ext_inst. intros. 
+  cases (ext l z) as E. assert (|-V' Some v ∶ t) as V. rewr_assumption. eauto.
+  inversion V. auto. destruct H0;auto.
+Qed.
+
+Hint Resolve mk_ext_inst_ext_inst mk_env_inst_env_inst mk_ext_inst_typed mk_env_inst_typed : inst.
+
+Lemma red_empty tis ti ext env c c' t' : 
+  Time 0 < ti -> TypeEnvP (map type tis) env -> TypeExtP ext -> TiTyC tis ti c -> 
+  Red c env ext c' t' -> t' = empty_trans.
+Proof.
+  intros L Tv Tx Tc R.
+  rewrite TiTyC_decompose in Tc. destruct Tc as [Tc1 Tc2].
+  inversion L. subst.
+  pose Tc1 as Tc1'.
+  apply Csem_typed_total 
+  with (env := mk_env_inst (map type tis) env)
+       (ext := mk_ext_inst ext) in Tc1';
+    eauto with inst. 
+  unfold total_trace in *. destruct Tc1' as [t Tc1'].
+  pose Tc1' as S.
+  eapply red_sound1 in S;eauto with inst.
+  eapply CausalC_empty in Tc1';eauto. rewrite Tc1' in S. auto. simpl. auto.
+Qed.
+
+Lemma tle_tlt x y z: x <= y -> y < z -> x < z.
+Proof.
+  intros X Y. destruct X. destruct Y; constructor. inversion Y;subst. inversion Y. subst.
+  constructor. omega.
+Qed.
+
+Theorem red_complete ti ti' tis c env ext : 
+  Time 0 <= ti -> TiTyC tis ti' c
+  -> ext_def_until ext ti -> env_def_until env tis ti -> TypeExtP ext -> TypeEnvP (map type tis) env
+  -> exists c' t', Red c env ext c' t'.
+Proof.
+  intros Ti T Ex Ev Te Tv.
+  generalize dependent env. generalize dependent ext. 
+  induction T; simpl; intros;eauto.
+  - (* Translate *)
+    destruct d; eauto.
+    assert (exists c' t', Red c env ext c' t') as IH by
+        (eapply IHT; try rewrite tsub'_0;try rewrite map_sub_time_0;eauto).
+    decompose [ex] IH. do 2 eexists. eauto. 
+  - (* Let *)
+    assert (exists c' t', Red c (fromLit (specialiseExp e env ext) :: env) ext c' t') as IH
+    by (eapply IHT;eauto; constructor;eauto using specialiseExp_complete;
+        rewrite TiTyE_decompose in H; destruct H; eauto using fromLit_typed,specialiseExp_typed).
+    decompose [ex] IH. do 2 eexists. econstructor;eauto.
+  - (* Scale *)
+    assert (exists c' t', Red c env ext c' t') as IH by (eapply IHT;eauto).
+    decompose [ex] IH.
+    cases (ti0 <=? ti) as TL.
+    * rewrite tleb_tle in TL.
+      eapply specialiseExp_complete in H;eauto.
+      apply fromLit_fromRLit in H. decompose [ex] H.
+      do 2 eexists. econstructor;eauto.
+      rewr_assumption. constructor.
+    * rewrite tleb_tgt in TL.
+      assert (Time 0 < ti0) as Ti' by eauto using tle_tlt.
+      assert (x0 = empty_trans) as Em. 
+      eauto using red_empty. subst.
+      do 2 eexists. econstructor;eauto.
+      eapply scaleTrans_empty.
+  - (* Both *)
+    assert (exists c' t', Red c1 env ext c' t') as IH1 by (eapply IHT1;eauto).
+    assert (exists c' t', Red c2 env ext c' t') as IH2 by (eapply IHT2;eauto).
+    decompose [ex] IH1. decompose [ex] IH2. eauto.
+  - (* If *)
+    eapply specialiseExp_complete in H;simpl;eauto. 
+    apply fromLit_fromBLit in H. destruct H as [b H].
+    destruct b. 
+    + assert (exists c' t', Red c1 env ext c' t') as IH1 by (eapply IHT1;eauto).
+      decompose [ex] IH1. eapply red_if_true in H;eauto.
+    + destruct d.
+      * assert (exists c' t', Red c2 env ext c' t') as IH2 by
+          (eapply IHT2;try rewrite tsub'_0;try rewrite map_sub_time_0;eauto). 
+        decompose [ex] IH2.
+        eapply red_if0_false in H;eauto.
+      * eapply red_ifS_false in H;eauto.
+Qed.
+
+
+Open Scope R.
+Import SMap.
+
+Definition lift2M {A B C} (f : A -> B -> C) (x : option (A * B)) : option C 
+  := liftM (fun x: (A * B) => let (x1,x2) := x in f x1 x2) x.
+
+
+
+Program Definition scale_trans' (v : option R) (t : SMap) : option SMap :=
+  match v with
+  | None => if SMap.is_empty t then Some SMap.empty else None
+  | Some v => Some (if Req_dec v 0 then SMap.empty else  SMap.map (fun x => v * x) _ t)
   end.
 
-Lemma redfun_red c env ext c' t : RedFun c env ext = Some (c', t) -> Red c env ext c' t.
+Next Obligation. 
+apply Rmult_integral in H0. destruct H0. tryfalse. assumption.
+Qed.  
+  
+
+
+
+(* Computable function that implements the reduction semantics. *)
+
+Fixpoint redfun (c : Contr) (env : EnvP) (ext : ExtEnvP) : option (Contr * SMap) :=
+  match c with
+    | Zero => Some (Zero, SMap.empty)
+    | Let e c => let e' := specialiseExp e env ext in
+                 liftM (fun ct : Contr * SMap => let (c', t) := ct in (smartLet (translateExp (-1) e') c', t)) 
+                       (redfun c (fromLit e'::env) ext)
+    | Transfer c p1 p2 => Some (Zero, SMap.singleton c p1 p2 1 R1_neq_R0)
+    | Scale e c => let e' := specialiseExp e env ext
+                   in redfun c env ext  >>= 
+                      (fun ct => let (c', t) := ct in 
+                                 liftM (fun t' => (smartScale (translateExp (-1) e') c', t'))
+                                       (scale_trans' (fromRLit e') t))
+    | Translate n c => match n with
+                         | O => redfun c env ext
+                         | S n' => Some (Translate n' c, SMap.empty)
+                       end
+    | Both c1 c2 =>  liftM2 (fun (ct1 ct2 : Contr * SMap) => let (c1',t1) := ct1 in 
+                                     let (c2',t2) := ct2 
+                                     in (smartBoth c1' c2', SMap.union_with Rplus t1 t2))
+                         (redfun c1 env ext) (redfun c2 env ext)
+    | If b n c1 c2 => fromBLit (specialiseExp b env ext) >>=
+                               (fun b' => if b' then redfun c1 env ext 
+                                          else match n with
+                                                 | O => redfun c2 env ext 
+                                                 | S n' => Some (If b n' c1 c2,SMap.empty)
+                                               end)
+  end.
+
+
+Definition smap_fun (m:SMap) (p1 p2 : Party) (a : Asset) : R := SMap.find p1 p2 a m.
+Definition smap_fun_eq (m:SMap) f := forall p1 p2 a, SMap.find p1 p2 a m = f p1 p2 a.
+
+Lemma smap_fun_empty : smap_fun SMap.empty = empty_trans.
 Proof.
-  generalize dependent c'. generalize dependent t. generalize dependent env.
-  induction c; intros env t c' R; simpl in R; try solve [inversion R;auto].
-  - option_inv_auto. destruct x0. apply IHc in H2. inversion H3.
-    eauto.
-  - remember (RedFun c env ext) as RF. destruct RF. destruct p. 
-    remember (E[|e|]env ext) as RS. destruct RS. destruct v. inversion R.
-    inversion R. auto. inversion R. inversion R.
-  - destruct n. auto. inversion R. auto.
-  - specialize IHc1 with (env:=env). specialize IHc2 with (env:=env). 
-    destruct (RedFun c1 env ext) as [p1| ]. destruct (RedFun c2 env ext) as [p2| ].
-    destruct p1, p2. inversion R. auto. destruct p1. inversion R. inversion R.
-  - remember (E[|e|] env ext) as BS. destruct BS. destruct v. destruct b. constructor; auto.
-    destruct n. constructor; auto. inversion R. constructor; auto. inversion R.
-    inversion R.
+ do 3 (apply functional_extensionality;intro). unfold smap_fun.
+ rewrite empty_find. reflexivity.
+Qed.
+
+Ltac eqb_eq := repeat rewrite andb_true_iff in *;repeat rewrite Party.eqb_eq in *; repeat rewrite Asset.eqb_eq in *.
+Ltac eqb_refl := repeat rewrite Party.eqb_refl in *; repeat rewrite Asset.eqb_refl in *.
+
+Lemma smap_fun_singleton p1 p2 a r p : smap_fun (singleton p1 p2 a r p) = singleton_trans p1 p2 a r.
+Proof.
+  unfold singleton_trans, smap_fun,find,singleton.
+  do 3 (apply functional_extensionality;intro).
+  cases (compare x x0) as C1. cases (Party.eqb p1 p2) as P1. reflexivity.
+  rewrite compare_eq in C1. subst. 
+  cases (Party.eqb p1 x0 && Party.eqb p2 x0 && Asset.eqb a x1) as E1.
+  eqb_eq. decompose [and] E1. subst. rewrite Party.eqb_refl in P1.
+  tryfalse. reflexivity.
+  cases (Party.eqb p1 p2) as P1;simpl. rewrite Party.eqb_eq in P1. rewrite <- compare_eq in P1.
+  rewrite P1. rewrite FMap.empty_find. reflexivity. 
+  cases (compare p1 p2) as C2. rewrite compare_eq in C2. subst. rewrite Party.eqb_refl in P1. tryfalse.
+  cases (FMap.find (x, x0, x1) (FMap.singleton (p1, p2, a) r)) as F1.
+  apply FMap.find_singleton in F1. destruct F1 as [F1 F1']. inversion F1. subst.
+  eqb_refl. reflexivity.  apply FMap.find_singleton_not in F1.
+  cases (Party.eqb p1 x && Party.eqb p2 x0 && Asset.eqb a x1) as E1.
+  eqb_eq. decompose [and] E1. subst. tryfalse.
+  cases (Party.eqb p1 x0 && Party.eqb p2 x && Asset.eqb a x1) as E2.
+  eqb_eq. decompose [and] E2. subst. rewrite compare_lt_gt in C1. tryfalse. reflexivity.
+  cases (FMap.find (x, x0, x1) (FMap.singleton (p1, p2, a) (- r))) as F1.
+  apply FMap.find_singleton in F1. destruct F1 as [F1 F1']. inversion F1. subst.
+  tryfalse. apply FMap.find_singleton_not in F1.
+  cases (Party.eqb p1 x && Party.eqb p2 x0 && Asset.eqb a x1) as E1.
+  eqb_eq. decompose [and] E1. subst. tryfalse.
+  cases (Party.eqb p1 x0 && Party.eqb p2 x && Asset.eqb a x1) as E2.
+  eqb_eq. decompose [and] E2. subst. unfold FMap.singleton. 
+  rewrite FMap.add_find_new. reflexivity.
+  cases (FMap.find (x, x0, x1) (FMap.singleton (p2, p1, a) (- r))) as F2.
+  apply FMap.find_singleton in F2. destruct F2. inversion H. subst.
+  eqb_refl. tryfalse. reflexivity.
+  
+  rewrite <- compare_lt_gt in C1.
+  cases (Party.eqb p1 p2) as P1;simpl. rewrite Party.eqb_eq in P1. rewrite <- compare_eq in P1.
+  rewrite P1. rewrite FMap.empty_find. reflexivity. 
+  cases (compare p1 p2) as C2. rewrite compare_eq in C2. subst. rewrite Party.eqb_refl in P1. tryfalse.
+  cases (FMap.find (x0, x, x1) (FMap.singleton (p1, p2, a) r)) as F1.
+  apply FMap.find_singleton in F1. destruct F1 as [F1 F1']. inversion F1. subst.
+  cases (Party.eqb x0 x && Party.eqb x x0 && Asset.eqb x1 x1) as E1.
+  eqb_eq. decompose [and] E1. subst x. rewrite <- compare_eq in H2. tryfalse.
+  cases (Party.eqb x0 x0 && Party.eqb x x && Asset.eqb x1 x1). reflexivity.
+  eqb_refl. tryfalse. apply FMap.find_singleton_not in F1.
+  cases (Party.eqb p1 x && Party.eqb p2 x0 && Asset.eqb a x1) as E1. eqb_eq.
+  decompose [and] E1. subst. rewrite compare_lt_gt in C1. tryfalse.
+  cases (Party.eqb p1 x0 && Party.eqb p2 x && Asset.eqb a x1) as E2. eqb_eq. 
+  decompose [and] E2. subst. tryfalse. reflexivity.
+  cases (FMap.find (x0, x, x1) (FMap.singleton (p2, p1, a) (- r))) as F1.
+  apply FMap.find_singleton in F1. destruct F1 as [F1 F1']. inversion F1. subst.
+  eqb_refl. simpl. apply Ropp_involutive.
+  apply FMap.find_singleton_not in F1.
+  cases (Party.eqb p1 x && Party.eqb p2 x0 && Asset.eqb a x1) as E1. eqb_eq.
+  decompose [and] E1. subst. tryfalse. 
+  cases (Party.eqb p1 x0 && Party.eqb p2 x && Asset.eqb a x1) as E2. eqb_eq.
+  decompose [and] E2. subst. tryfalse. reflexivity.
+Qed.
+
+Hint Constructors Red.
+
+Ltac dprod := repeat match goal with
+                       | [_: context[let (_,_) := ?x in _] |- _] => is_var x; destruct x
+                       | [T: (_,_)=(_,_) |- _] => inversion T;clear T
+                     end.
+
+Lemma scale_trans_ScaleTrans (v : option R) t t' m m' : 
+  t' = smap_fun m' -> t = smap_fun m -> scale_trans' v m = Some m' -> ScaleTrans v t t'.
+Proof.
+  intros. destruct v. simpl in H1. inversion H1;clear H1. assert (t' = scale_trans r t) as S.
+  subst. unfold smap_fun, scale_trans. repeat (apply functional_extensionality;intro).
+  cases (Req_dec r 0) as E. rewrite empty_find. subst. 
+  rewrite Rmult_0_r. reflexivity.
+  rewrite map_find. apply Rmult_comm. apply Rmult_0_r. intros. rewrite Ropp_mult_distr_r_reverse.
+  reflexivity. rewrite S. econstructor.
+  simpl in H1. cases (is_empty m) as R. inversion H1.
+  rewrite empty_is_empty in R. subst. rewrite smap_fun_empty. constructor.
+  tryfalse.
+Qed.
+
+Lemma smap_fun_add m1 m2 :  smap_fun (union_with Rplus m1 m2) = add_trans (smap_fun m1) (smap_fun m2).
+Proof.
+  unfold smap_fun, add_trans. repeat (apply functional_extensionality;intro). apply union_find.
 Qed.
 
 
-Lemma red_redfun c env ext c' t : Red c env ext c' t -> RedFun c env ext = Some (c', t).
+Theorem redfun_red c c' env ext t: 
+  redfun c env ext = Some (c', t) -> Red c env ext c' (smap_fun t) .
 Proof.
-  intros R. induction R; simpl; repeat (simpl;rewr_assumption); auto. 
+  intro F. generalize dependent t. generalize dependent c'. 
+  generalize dependent ext. generalize dependent env. 
+  induction c;intros;simpl in *;try first[option_inv' F|injection F;intros];dprod;option_inv_auto;dprod;subst;
+  eauto using smap_fun_empty, smap_fun_singleton, scale_trans_ScaleTrans, smap_fun_add.
+  - destruct n; inversion F; auto using smap_fun_empty.
+  - destruct x. auto. destruct n. auto. inversion H2. auto using smap_fun_empty.
 Qed.
 
-Theorem Red_function c env ext c' t : RedFun c env ext = Some (c', t) <-> Red c env ext c' t.
-Proof. split. apply redfun_red. apply red_redfun. Qed.
+
+Lemma smap_fun_empty_compact m : smap_fun m = empty_trans -> m = SMap.empty.
+Proof.
+  destruct m as [M C]. intro F. 
+  apply empty_find_compact;eauto. intros.
+  do 3 eapply equal_f in F.
+  unfold smap_fun in F. rewrite F. reflexivity.
+Qed.
+
+
+Lemma ScaleTrans_scale_trans (v : option R) t t' m : 
+  t = smap_fun m -> ScaleTrans v t t' -> exists m', scale_trans' v m = Some m' /\ t' = smap_fun m'.
+Proof.
+  intros T S. inversion S. 
+  - subst. symmetry in H0. apply smap_fun_empty_compact in H0;auto.
+    eexists. split. destruct v. simpl. cases (Req_dec r 0). reflexivity.
+    rewrite -> H0. rewrite SMap.map_empty. reflexivity. simpl.
+    cases (is_empty m). reflexivity. rewrite <- SMap.empty_is_empty in H0. tryfalse.
+    rewrite smap_fun_empty. reflexivity.
+  - simpl. cases (Req_dec v0 0) as R. 
+    eexists. split. reflexivity. subst.
+    rewrite scale_trans_0. rewrite smap_fun_empty. reflexivity.
+    eexists. split. reflexivity. subst. unfold smap_fun, scale_trans.
+    do 3 (apply functional_extensionality;intro). rewrite map_find. apply Rmult_comm.
+    apply Rmult_0_r. intros. rewrite Ropp_mult_distr_r_reverse. reflexivity.
+Qed.
+
+
+Theorem red_redfun c c' env ext t: 
+  Red c env ext c' t -> exists m, redfun c env ext = Some (c', m) /\ smap_fun m = t.
+Proof.
+  intro F. induction F; subst; 
+  repeat match goal with | [T : exists _, _ /\ _ |- _] => decompose [ex and] T; clear T;subst end;
+  try solve[eexists;split;simpl;try reflexivity;eauto using smap_fun_empty,smap_fun_singleton, smap_fun_add;
+  repeat match goal with | [T : _ = Some _ |- _] => rewrite T; clear T end; 
+  simpl;unfold pure,compose;simpl;try reflexivity].
+  (* we only need to deal with scale *)
+  - eapply ScaleTrans_scale_trans in H0. decompose [ex and] H0.
+    eexists. split. simpl. rewrite H1. simpl.
+    rewrite H3. simpl.
+    unfold pure, compose. rewrite H2. reflexivity. auto. eauto. 
+  Qed.
+
+
+
